\documentclass[a0paper, landscape]{paper}
\usepackage{../mathpartir}
\usepackage[margin=0.5cm]{geometry}
\input{../while}
\begin{document}

\section*{2.3:}

\[
\inferrule*[left=\rcompns, width=\textwidth]{ 
  \inferrule*[left=\rassns]{ }{\ns {\cass x 3} {[]} {[x\mapsto 3]}}\\
  \inferrule*[left=\rcompns]{ 
    \inferrule*[left=\rassns]{ }{\ns {\cass y 0} {[x\mapsto 3]} {[x\mapsto 3,\; y\mapsto 0]}}\\
    \inferrule*[left=\rwhilettns, width=\textwidth, right=\ensuremath{\beval {\neg(\cvar{x}\le 0)} {[x\mapsto 3,\; y\mapsto 0]}=\ltrue}]{
      \inferrule*[left=\rcompns]{ 
        \inferrule*[left=\rassns]{ }{\ns {\cass y {\cvar y + \cvar x}} {[x\mapsto 3,\; y\mapsto 0]} {[x\mapsto 3,\; y\mapsto 3]}} \\
        \inferrule*[left=\rassns]{ }{\ns {\cass x {\cvar x - 1}} {[x\mapsto 3,\; y\mapsto 3]} {[x\mapsto 2,\; y\mapsto 3]}}
      }{\ns D {[x\mapsto 3,\; y\mapsto 0]} {[x\mapsto 2,\; y\mapsto 3]}} \\
       {\inferrule*[left=\rwhilettns, width=\textwidth, right=\ensuremath{\beval {\neg(\cvar{x}\le 0)} {[x\mapsto 2,\; y\mapsto 3]}=\ltrue}]{
           \inferrule*[left=\rcompns]{ 
             \inferrule*[left=\rassns]{ }{\ns {\cass y {\cvar y + \cvar x}} {[x\mapsto 2,\; y\mapsto 3]} {[x\mapsto 2,\; y\mapsto 5]}} \\
             \inferrule*[left=\rassns]{ }{\ns {\cass x {\cvar x - 1}} {[x\mapsto 2,\; y\mapsto 5]} {[x\mapsto 1,\; y\mapsto 5]}}
           }{\ns D {[x\mapsto 2,\; y\mapsto 3]} {[x\mapsto 1,\; y\mapsto 5]}} \\
                      {\inferrule*[left=\ensuremath{T_3\quad=\quad}\rwhilettns, width=\textwidth, right=\ensuremath{\beval {\neg(\cvar{x}\le 0)} {[x\mapsto 1,\; y\mapsto 5]}=\ltrue}]{
  \inferrule*[left=\rcompns]{ 
    \inferrule*[left=\rassns]{ }{\ns {\cass y {\cvar y + \cvar x}} {[x\mapsto 1,\; y\mapsto 5]} {[x\mapsto 1,\; y\mapsto 6]}} \\
    \inferrule*[left=\rassns]{ }{\ns {\cass x {\cvar x - 1}} {[x\mapsto 1,\; y\mapsto 6]} {[x\mapsto 0,\; y\mapsto 6]}}
  }{\ns D {[x\mapsto 1,\; y\mapsto 5]} {[x\mapsto 0,\; y\mapsto 6]}} \\
  {\inferrule*[left=\rwhileffns, right=\ensuremath{\beval {\neg(\cvar{x}\le 0)} {[x\mapsto 0,\; y\mapsto 6]}=\lfalse}]{ }{\ns C {[x\mapsto 0,\; y\mapsto 6]} {[x\mapsto 0,\; y\mapsto 6]}}}
}{\ns C {[x\mapsto 1,\; y\mapsto 5]} {[x\mapsto 0,\; y\mapsto 6]}}
}
         }{\ns C {[x\mapsto 2,\; y\mapsto 3]} {[x\mapsto 0,\; y\mapsto 6]}}
       }
    }{\ns C {[x\mapsto 3,\; y\mapsto 0]} {[x\mapsto 0,\; y\mapsto 6]}}    
  }{\ns B {[x\mapsto 3]} {[x\mapsto 0,\; y\mapsto 6]}}
}{\ns A {[]} {[x\mapsto 0,\; y\mapsto 6]}}
\]

\section*{2.4:}
Do the following statements terminate:\\
\cwhile {\neg(\cvar{x}= 1)} (\ccomp {\cass y y*x} {\cass x x-1}) \\

\cwhile {1\le \cvar{x}} (\ccomp {\cass y y*x} {\cass x x-1}) \\

\cwhile {true}  \cskip \\

\section*{2.6:}
Show that $S1;(S2;S3)$ and $(S1;S2);S3$ are semantically equivalent: \\

Show that $S1;S2$ and $S2;S1$ are not always semantically equivalent:



\section*{2.7:}
While can be extended with the:
 \crepeat S b statement:

\section*{2.8:}

\end{document}