\documentclass{article}
\usepackage[margin=0.5cm]{geometry}
\usepackage[utf8]{inputenc}
\usepackage{graphicx}
\usepackage{listings}
\usepackage{color}
\usepackage{placeins}
\usepackage{hyperref}
\usepackage{xcolor}
\usepackage{caption}
\usepackage{amsfonts}

\begin{document}

\include{frontpage}

\section*{Putting it all Together:}
Recursive equations:\\
$a = A()	$\\
$b = B(a) 	$\\
$c = C(b)	$\\
$d = D(c,\;e) $\\
$e = E(d)	$\\
$f = F(e)	$\\

\noindent Transfer functions:\\
$A = [\bot,\;\bot] $\\
$B = \lambda E.\;E[x \mapsto +]$\\
$C = \lambda E.\;E[y \mapsto 0]$\\
$D = \lambda E.\;\lambda E'.\;E\sqcup E'$\\
$E = \lambda E.\;E[x \mapsto E[y],\;y\mapsto E[x]]$\\
$F = \lambda E.\;E[y \mapsto E[y] \oplus\;+]$\\

\noindent Big transfer function:
$$T(a ,b ,c, d, e, f)\;=\;([\bot,\;\bot],\;a[x\mapsto+],\;b[y\mapsto 0],\;c\sqcup e,\;(d[x \mapsto d[y],\;y\mapsto d[x]]),\;e[y \mapsto e[y] \oplus\;+])$$

\noindent Finding least fixed:
\begin{enumerate}
	\item $([\bot,\;\bot],	[\bot,\;\bot], 	[\bot,\;\bot], 	[\bot,\;\bot], 	[\bot,\;\bot], 	[\bot,\;\bot])$
	\item $([\bot,\;\bot], 	[+,\;\bot], 	[\bot,\;0], 	[\bot,\;\bot],  [\bot,\;\bot],  [\bot,\;\bot])$
	\item $([\bot,\;\bot], 	[+,\;\bot], 	[+,\;0], 	[\bot,\;0], 	[\bot,\;\bot], 	[\bot,\;\bot])$
	\item $([\bot,\;\bot], 	[+,\;\bot], 	[+,\;0], 	[+,\;0], 	[0,\;\bot], 	[0,\;\bot])$
	\item $([\bot,\;\bot], 	[+,\;\bot], 	[+,\;0], 	[0+,\;0], 	[0,\;+], 	[0,\;\bot])$
	\item $([\bot,\;\bot], 	[+,\;\bot], 	[+,\;0], 	[0+,\;0+], 	[0,\;0+], 	[0,\;+])$

	\item $([\bot,\;\bot], 	[+,\;\bot], 	[+,\;0], 	[0+,\;0+], 	[0+,\;0+], 	[0,\;0+])$

	\item $([\bot,\;\bot], 	[+,\;\bot], 	[+,\;0], 	[0+,\;0+], 	[\bot,\;\bot], 	[\bot,\;\bot])$

	\item $([\bot,\;\bot], 	[+,\;\bot], 	[+,\;0], 	[0+,\;0+], 	[\bot,\;\bot], 	[\bot,\;\bot])$
\end{enumerate}

\section*{Monotone Functions and Fixed-Points:}

\subsection*{i)}
$$X\;=\;\{a,\;b\}$$
$$Y\;=\;X\cup Y$$
In equation form:
$$X\;=\;f(X, Y)\;=\;\{a,\;b\}$$
$$Y\;=\;g(X, Y)\;=\;X\cup Y$$
Can be written as:
$$X\;=\;f()\;=\;\{a,\;b\}$$
$$Y\;=\;g(X, Y)\;=\;X\cup Y$$
The function $f()$ is monotone, as it is constant. Therefore $f() \sqsubseteq f()$ will always hold. The function $g(X,\;Y)$ is also monotone, as no matter which sets use give the function it will combine them and the resulting set will always be greater or equal to the input sets.

\subsection*{ii)}
$$X\;=\;\{a,\;b\}\cup Y$$
$$Y\;=\;X\;\setminus\;\{b\}$$
In equation form:
$$X\;=\;f(X, Y)\;=\;\{a,\;b\}\cup Y$$
$$Y\;=\;g(X, Y)\;=\;X\;\setminus\;\{b\}$$
Can be written as:
$$X\;=\;f(Y)\;=\;\{a,\;b\}\cup Y$$
$$Y\;=\;g(X)\;=\;X\;\setminus\;\{b\}$$
The function $f(Y)$ is monotone, as it return $\{a,\;b\}\cup Y$ which is always a superset of $Y$. The function $g(X)$ is also monotone. It is hard to give an example of why, however intuitively removing a constant element preserves monotonicity, as the same element is removed on both sides of $\sqsubseteq$.
\subsection*{iii)}
$$X\;=\;\{a,\;b\}\cup Z$$
$$Y\;=\;\{a,\;c\}\setminus X$$
$$Z\;=\;X^C$$
In equation form:
$$X\;=\;f(X,\;Y,\;Z)\;=\;\{a,\;b\}\cup Z$$
$$Y\;=\;g(X,\;Y,\;Z)\;=\;\{a,\;c\}\setminus X$$
$$Z\;=\;h(X,\;Y,\;Z)\;=\;X^C$$
Can be written as:
$$X\;=\;f(Z)\;=\;\{a,\;b\}\cup Z$$
$$Y\;=\;g(X)\;=\;\{a,\;c\}\setminus X$$
$$Z\;=\;h(X)\;=\;X^C$$
The function $f(Z)$ is monotone, as it return $\{a,\;b\}\cup Z$ which is always a superset of $Z$. If $g(X)$ is monotone then $\forall\;Y,\;Y'\;P(\{a,\;b,\;c\}):\;Y\;\sqsubseteq\;Y'$. However this is not the case:
$$\emptyset\sqsubseteq \{a,\;b,\;c\}$$
$$g(\emptyset)\not\sqsubseteq g(\{a,\;b,\;c\})$$
$$\{a,\;c\}\not\sqsubseteq \emptyset$$
$g(X)$ is therefore not monotone. $h(X)$ is not monotone either, as:
$$\emptyset\sqsubseteq \{a,\;b,\;c\}$$
$$g(\emptyset)\not\sqsubseteq g(\{a,\;b,\;c\})$$
$$\{a,\;b\;c\}\not\sqsubseteq \emptyset$$
\end{document}
